{"cells":[{"cell_type":"markdown","metadata":{},"source":["- KEYWORDS: System, Discretization, z-transform\n"]},{"cell_type":"code","execution_count":1,"metadata":{},"outputs":[{"name":"stdout","output_type":"stream","text":"# Out[0]:"}],"source":[""]},{"cell_type":"markdown","metadata":{},"source":["## Impulse Response Representation of DT Systems\n\n"]},{"cell_type":"markdown","metadata":{},"source":["In previous section, we introduced that a DT system can be represented by its inputs and outputs. In the input-output representation, we know that the output of a system can be determined by its previous outputs and inputs. In that representation, we need to know all the inputs and all the previous outputs. Sometimes, this is not convenient. In this section, we introduce another important DT system representation: impulse response representation. Using this representation, we can determine the output of a system directly (without evaluating the previous outputs) for any given input sequence.\n\n"]},{"cell_type":"markdown","metadata":{},"source":["### Impulse response\n\n"]},{"cell_type":"markdown","metadata":{},"source":["First, we need to introduce impulse response. The impulse response $h(n)$ of an linear time-invariant (LTI) system $T$ is defined as the response of the system to the unit impulse (or sample) signal $\\delta(n)$:\n\n$$h(n) = T\\{\\delta(n)\\} $$\n\n"]},{"cell_type":"markdown","metadata":{},"source":["### Response of LTI DT systems\n\n"]},{"cell_type":"markdown","metadata":{},"source":["Note that in this section, we again assume the system has zero initial condition (i.e., $y(n)=0$ for $n < 0$ ). Recall that the sequence of any arbitrary signal can be represented as:\n\n$$x(n) = \\sum_{k=-\\infty}^{\\infty}x(k)\\delta(n-k)$$\n\nSince the system we consider is time-invariant, if\n\n$$h(n)=T\\{\\delta(n)\\}$$\n\nThen,\n\n$$T\\{\\delta(n-k)\\}=h(n-k)$$\n\nfor any $k$. Furthermore, the system is linear,\n\n$$\\begin{array}{ccc} y(n) & = & T \\{x(n)\\} = T\\{\\sum_{k=-\\infty}^{\\infty}x(k)\\delta(n-k)\\}\\\\ &=& \\sum_{k=-\\infty}^{\\infty}T\\{x(k)\\delta(n-k)\\}\\\\ &=&\\sum_{k=-\\infty}^{\\infty}x(k)T\\{\\delta(n-k)\\}  \\end{array} $$\n\nFrom the above equations, we can obtain that the response of the system to the input sequence $x$ is:\n\n$$y(n) = \\sum_{k=-\\infty}^{\\infty}x(k)h(n-k)\\tag{0}\\label{eqn:ch2:convolution}$$\n\nFor causal systems, the above equation can be simplified:\n\n$$y(n) = \\sum_{k=-\\infty}^{n}x(k)h(n-k)\\tag{1}\\label{eqn:ch2:convolution1}$$\n\nThis implies that the response of an LTI system to an arbitrary input sequence can be calculated using the system's impulse response. Equation~(\\ref{eqn:ch2:convolution}) is also called the *convolution sum* of the $x$ and $h$. This operation is denoted by $*$. That is,\n\n$$y(n) = \\sum_{k=-\\infty}^{n}x(k)h(n-k) = x(n)*h(n)\\tag{2}\\label{eqn:ch2:convolution2}$$\n\nThe operation of convolution is {\\em commutable} which means:\n\n$$y(n)=x(n)*h(n) = h(n)*x(n) =\\displaystyle\\sum_{k=0}^{\\infty}h(k)x(n-k)\\tag{3}\\label{eqn:ch2:convolution3}$$\n\nTo summarize, the response of an LTI system to an arbitrary input sequence can be calculated using the convolution sum of the input sequence and the system's impulse response.\n\n"]},{"cell_type":"markdown","metadata":{},"source":["### Example\n\n"]},{"cell_type":"markdown","metadata":{},"source":["Suppose that the impulse response of a causal LTI system is:\n\n$$\\begin{array}{rcl}h(n)=\\{\\hspace{-3mm}&1&\\hspace{-3mm},2,1,-1\\}\\\\&\\uparrow&\\end{array}$$\nDetermine its response to:\n\n$$\\begin{array}{rcl}x(n)=\\{\\hspace{-3mm}&1&\\hspace{-3mm},2,3,1\\}\\\\&\\uparrow&\\end{array}$$\n\nNote that these are sequences of values starting from $n=0$ and the arrow indicates the time instant $n=0$. If no arrow is used, it means the first value corresponds to $n=0$.\n\nUsing convolution sum, we can write that:\n\n$$y(n) = x(n)*h(n) = \\sum_{k=-\\infty}^{n}x(k)h(n-k)$$\n\nFrom the definitions of $h$ and $x$, it can be seen that for $ n<0$ and $n\\geq 4$, the signals are not defined. In this course, we will treat these undefined values as zero. Strictly speaking, \\`undefined' and \\`zero' are two different things. However, treating \\`undefined' as zero, greatly simplifies the calculation of convolution sum and all the other calculations in this course. Let us use the index of $x$ as a reference to determine the range of $k$ that should be considered. From the definition of $x$, we can find that we only have to consider $0\\leq k\\leq 3$. For all the other $k$, $x(k)$ will have a zero value. Therefore, the above equation can be simplified to the following:\n\n$$ y(n) = x(n)*h(n) = \\sum_{k=0}^{n}x(k)h(n-k)$$\nIf $n=0$, we have\n\n$$\\begin{array}{rcl}y(0) & = & \\sum_{k=0}^{0}x(k)h(-k)\\\\& = & x(0)h(0)\\\\& = & 1\\cdot 1\\\\& = & 1\\end{array}$$\n\nSimilarly, we can evaluate $y(1)$, $y(2)$, $\\cdots$\n\n$$\\begin{array}{rcl}y(1) & = & \\sum_{k=0}^{1}x(k)h(1-k)\\\\& = & x(0)h(1) + x(1)h(0)\\\\& = & 1\\cdot 2 + 2\\cdot 1\\\\& = & 4\\end{array}$$\n\n$$\\begin{array}{rcl}y(2) & = &\\sum_{k=0}^{2}x(k)h(2-k)\\\\& = & x(0)h(2) + x(1)h(1) + x(2)h(0)\\\\& = & 1\\cdot 1 + 2\\cdot 2 + 3\\cdot 1\\\\& = & 8\\end{array}$$\n\n$$\\begin{array}{rcl}y(3) & = &\\sum_{k=0}^{3}x(k)h(3-k)\\\\& = & x(0)h(3) + x(1)h(2) + x(2)h(1) + x(3)h(0)\\\\& = & 1\\cdot (-1) + 2\\cdot 1 + 3\\cdot 2 + 1\\cdot 1\\\\& = & 8\\end{array}$$\n\nThe output sequence is:\n\n$$y(n)=\\left\\{1,4,8,8,3,-2,-1\\right\\}$$\n\nRemark: Note that the convolution sum is based on zero initial condition of the system (i.e., $y(n)=0$ for $n<0$). When the initial condition is not zero, we need to consider the effects of the initial condition as well.\n\n"]},{"cell_type":"markdown","metadata":{},"source":["#### Example: Calculation of the convolution of two signals\n\n"]},{"cell_type":"code","execution_count":1,"metadata":{},"outputs":[{"name":"stdout","output_type":"stream","text":"fig1\n# Out[2]:\n: array([ 1,  4,  8,  8,  3, -2, -1])"}],"source":["%matplotlib inline\nimport matplotlib.pyplot as plt\nimport numpy as np\nimport math\n\nh=np.array([1,2,1,-1])\nx=np.array([1,2,3,1])\n\n\nnp.convolve(h,x)"]},{"cell_type":"markdown","metadata":{},"source":["### Causality condition\n\n"]},{"cell_type":"markdown","metadata":{},"source":["In the previous section, from eqn:ch2:convolution to eqn:ch2:convolution1, we simply used the fact that there should be no future inputs in the output of a causal system. If we look into eqn:ch2:convolution, we can find a condition for the causality of LTI systems. Let us write eqn:ch2:convolution into two parts as follows:\n\n$$y(n) =  \\sum_{k=-\\infty}^{\\infty}x(k)h(n-k) = \\displaystyle\\sum_{k=-\\infty}^{n}x(k)h(n-k)+\\displaystyle\\sum_{k=n+1}^{\\infty}x(k)h(n-k)\\tag{3}\\label{eqn:ch2:causality}$$\n\nFor a causal system, we know that the second term on the right should not appear since it involves all the future inputs. If we look at the corresponding $h$ values, we can find the second term including the following elements of $h$:\n\n$$h(-1),\\;h(-2),\\;h(-3),\\;\\ldots$$\n\nSince $x(k)$ for $k\\geq n$ could be arbitrary values, the condition that ensures causality of the system is:\n\n$$h(-1) = 0,\\;h(-2)=0,\\;h(-3)=0,\\ldots$$\n\nThat is:\n\n$$h(n)=0,\\;for\\; all\\;\\; n<0$$\n\nThis condition is actually a necessary and sufficient condition. To summarize the above result, an LTI system is causal if and only if its impulse response must be zero for $n<0$.\n\n"]},{"cell_type":"markdown","metadata":{},"source":["## Summary\n\n"]},{"cell_type":"markdown","metadata":{},"source":["-   We introduce impulse response\n    -   We calculate impulse response by convolution\n\n"]}],"metadata":{"org":{"KEYWORDS":"System, Discretization, z-transform"},"kernelspec":{"display_name":"Python 3","language":"python","name":"python3"},"language_info":{"codemirror_mode":{"name":"ipython","version":3},"file_extension":".py","mimetype":"text/x-python","name":"python","nbconvert_exporter":"python","pygments_lexer":"ipython3","version":"3.5.2"}},"nbformat":4,"nbformat_minor":0}